checker.v
@@ -1,0 +1,126 @@
+Require Import Arith.
+Require Import Nat.
+Require Import Bool.
+Require Import bbv.Word.
+Require Import List.
+Require Import Coq_EVM.optimizations.
+Import Optimizations.
+Require Import Coq_EVM.datatypes.
+Import EVM_Def Concrete Abstract Optimizations.
+Require Import Coq_EVM.interpreter.
+Import Interpreter SFS.
+Import ListNotations.
+
+Module Checker.
+
+Definition equiv_checker (p1 p2: prog) (height: nat) (opt: optimization) 
+  : bool :=
+match symbolic_exec p1 height opmap with
+| None => false
+| Some sfs1 => 
+    match symbolic_exec p2 height opmap with 
+    | None => false
+    | Some sfs2 => let (sfs3, _) := opt sfs2 in 
+                   asfs_eq sfs1 sfs3 opmap
+    end
+end.
+
+Lemma symb_exec''_strictly_decreasing: forall (ins: instr) (a a': asfs) 
+  (ops: opm),
+strictly_decreasing_map_asfs a ->
+symbolic_exec'' ins a ops = Some a' ->
+strictly_decreasing_map_asfs a'.
+Proof.
+intros. destruct ins eqn: eq_ins.
+- (*PUSH*)
+  admit.
+- (*POP*)
+  admit.
+- (*DUP*)
+  admit.
+- (*SWAP*)
+  admit.
+- (*Operation*)
+  admit.
+Admitted.
+
+Lemma symb_exec'_strictly_decreasing: forall (p: prog) (a a': asfs) 
+  (ops: opm),
+strictly_decreasing_map_asfs a ->
+symbolic_exec' p a ops = Some a' ->
+strictly_decreasing_map_asfs a'.
+Proof.
+induction p as [| ins rp IH].
+- intros. simpl in H0. injection H0 as eq_a_a'. 
+  rewrite <- eq_a_a'. assumption.
+- intros. simpl in H0. 
+  destruct (symbolic_exec'' ins a ops) as [a''|] 
+    eqn: eq_sym_exec''; try discriminate.
+  apply symb_exec''_strictly_decreasing in eq_sym_exec''; try assumption.
+  apply IH in H0; try assumption.
+Qed.
+
+Lemma decreasing_asfs_empty_asfs: forall (height: nat),
+strictly_decreasing_map_asfs (empty_asfs height).
+Proof.
+intros. simpl. auto.
+Qed.
+
+Lemma symb_exec_strictly_decreasing: forall (p: prog) (height: nat) (ops: opm)
+  (sfs: asfs),
+symbolic_exec p height ops = Some sfs ->
+strictly_decreasing_map_asfs sfs.
+Proof.
+intros.
+unfold symbolic_exec in H.
+apply symb_exec'_strictly_decreasing with (p:=p) (a:=empty_asfs height)
+  (ops:=ops).
+- apply decreasing_asfs_empty_asfs.
+- assumption.
+Qed.
+
+
+
+Theorem equiv_checker_correct: forall (p1 p2: prog) (height: nat) 
+  (opt: optimization) (in_es out_es1 out_es2: execution_state) 
+  (in_stk: concrete_stack),
+safe_optimization opt ->
+equiv_checker p1 p2 height opt = true ->
+get_stack_es in_es = in_stk ->
+length in_stk = height ->
+concr_interpreter p1 in_es opmap = Some out_es1 ->
+concr_interpreter p2 in_es opmap = Some out_es2 ->
+get_stack_es out_es1 = get_stack_es out_es2.
+Proof.
+intros.
+unfold equiv_checker in H0.
+destruct (symbolic_exec p1 height opmap) as [sfs1|] eqn: symb_exec_p1;
+  try discriminate.
+destruct (symbolic_exec p2 height opmap) as [sfs2|] eqn: symb_exec_p2;
+  try discriminate.
+destruct (opt sfs2) as [sfs3 flag] eqn: opt_sfs2.
+destruct out_es1 as [out_stk1 mem1 storage1] eqn: eq_out_es1.
+assert (get_stack_es out_es1 = out_stk1) as eq_get_stack_1;
+  try (rewrite -> eq_out_es1; auto).
+rewrite <- eq_out_es1 in H3.
+destruct out_es2 as [out_stk2 mem2 storage2] eqn: eq_out_es2.
+assert (get_stack_es out_es2 = out_stk2) as eq_get_stack_2;
+  try (rewrite -> eq_out_es2; auto).
+rewrite <- eq_out_es2 in H4.  
+simpl.
+pose proof (correctness_symb_exec p1 in_stk out_stk1 opmap height in_es
+  out_es1 sfs1 H2 H1 H3 eq_get_stack_1 symb_exec_p1) as Heval_sfs1.
+pose proof (correctness_symb_exec p2 in_stk out_stk2 opmap height in_es
+  out_es2 sfs2 H2 H1 H4 eq_get_stack_2 symb_exec_p2) as Heval_sfs2.
+pose proof (asfs_eq_correctness sfs1 sfs3 opmap in_stk H0) as eq_eval_sfs1_sfs3.
+unfold safe_optimization in H.
+apply symb_exec_strictly_decreasing in symb_exec_p2 as Hdecr_sfs2.
+pose proof (H in_stk out_stk2 sfs2 sfs3 flag Heval_sfs2 opt_sfs2 Hdecr_sfs2)
+ as [Heval_sfs3 _].
+rewrite -> Heval_sfs1 in eq_eval_sfs1_sfs3.
+rewrite -> Heval_sfs3 in eq_eval_sfs1_sfs3.
+injection eq_eval_sfs1_sfs3. auto.
+Qed.
+
+End Checker.
+Import Checker.
